pulse/lib/steel/pulse/Pulse.Typing.Metatheory.fsti
@@ -3,101 +3,34 @@ open Pulse.Syntax
 open Pulse.Syntax.Naming
 open Pulse.Typing
 
-let comp_typing_u (g:env) (c:comp_st) = comp_typing g c (comp_u c)
+include Pulse.Typing.Metatheory.Base
 
-val admit_comp_typing (g:env) (c:comp_st)
-  : comp_typing_u g c
-  
-val st_typing_correctness (#g:env) (#t:st_term) (#c:comp_st) 
-                          (_:st_typing g t c)
-  : comp_typing_u g c
+val tot_typing_weakening_single (#g:env) (#t #ty:term)
+  (d:tot_typing g t ty)
+  (x:var { ~ (x `Set.mem` dom g)})
+  (x_t:typ)
 
-val comp_typing_inversion (#g:env) (#c:comp_st) (ct:comp_typing_u g c)
-  : st_comp_typing g (st_comp_of_comp c)
-
-val st_comp_typing_inversion_cofinite (#g:env) (#st:_) (ct:st_comp_typing g st)
-  : (universe_of g st.res st.u &
-     tot_typing g st.pre tm_vprop &
-     (x:var{fresh_wrt x g (freevars st.post)} -> //this part is tricky, to get the quantification on x
-       tot_typing (push_binding g x ppname_default st.res) (open_term st.post x) tm_vprop))
-
-val st_comp_typing_inversion (#g:env) (#st:_) (ct:st_comp_typing g st)
-  : (universe_of g st.res st.u &
-     tot_typing g st.pre tm_vprop &
-     x:var{fresh_wrt x g (freevars st.post)} &
-     tot_typing (push_binding g x ppname_default st.res) (open_term st.post x) tm_vprop)
-
-val tm_exists_inversion (#g:env) (#u:universe) (#ty:term) (#p:term) 
-                        (_:tot_typing g (tm_exists_sl u (as_binder ty) p) tm_vprop)
-                        (x:var { fresh_wrt x g (freevars p) } )
-  : universe_of g ty u &
-    tot_typing (push_binding g x ppname_default ty) p tm_vprop
-
-val tot_typing_weakening (#g:env) (#t:term) (#ty:term)
-                         (x:var { fresh_wrt x g Set.empty })
-                         (x_t:typ)
-                         (_:tot_typing g t ty)
-   : tot_typing (push_binding g x ppname_default x_t) t ty
-
-val pure_typing_inversion (#g:env) (#p:term) (_:tot_typing g (tm_pure p) tm_vprop)
-   : tot_typing g p (tm_fstar FStar.Reflection.Typing.tm_prop Range.range_0)
-
-
-let comp_st_with_post (c:comp_st) (post:term) : c':comp_st { st_comp_of_comp c' == ({ st_comp_of_comp c with post} <: st_comp) } =
-  match c with
-  | C_ST st -> C_ST { st with post }
-  | C_STGhost i st -> C_STGhost i { st with post }
-  | C_STAtomic i st -> C_STAtomic i {st with post}
-
-let comp_st_with_pre (c:comp_st) (pre:term) : comp_st =
-  match c with
-  | C_ST st -> C_ST { st with pre }
-  | C_STGhost i st -> C_STGhost i { st with pre }
-  | C_STAtomic i st -> C_STAtomic i {st with pre }
-
-let pairwise_disjoint (g g' g'':env) =
-  disjoint g g' /\ disjoint g' g'' /\ disjoint g g''
+  : tot_typing (push_binding g x ppname_default x_t) t ty
 
 val st_typing_weakening
   (g:env) (g':env { disjoint g g' })
-  (t:st_term) (c:comp) (_:st_typing (push_env g g') t c)
-  (g1:env { pairwise_disjoint g g1 g' })
-  : st_typing (push_env (push_env g g1) g') t c
+  (t:st_term) (c:comp) (d:st_typing (push_env g g') t c)
+  (g1:env { g1 `env_extends` g /\ disjoint g1 g' })
+  : st_typing (push_env g1 g') t c
 
-let veq_weakening
+val st_typing_weakening_standard
+  (#g:env) (#t:st_term) (#c:comp) (d:st_typing g t c)
+  (g1:env { g1 `env_extends` g })
+  : st_typing g1 t c
+
+val st_typing_weakening_end
   (g:env) (g':env { disjoint g g' })
-  (#v1 #v2:vprop) (_:vprop_equiv (push_env g g') v1 v2)
-  (g1:env { pairwise_disjoint g g1 g' })
-  : vprop_equiv (push_env (push_env g g1) g') v1 v2 = magic ()
+  (t:st_term) (c:comp) (d:st_typing (push_env g g') t c)
+  (g'':env { g'' `env_extends` g' /\ disjoint g'' g })
+  : st_typing (push_env g g'') t c
 
-// move to Env
-let singleton_env (f:_) (x:var) (t:typ) = push_binding (mk_env f) x ppname_default t
-
-let nt (x:var) (t:term) = [ NT x t ]
-
-val subst_env (en:env) (ss:subst)
-  : en':env { fstar_env en == fstar_env en' /\
-              dom en == dom en' }
-
-val st_typing_subst
-  (g:env) (x:var) (t:typ) (g':env { pairwise_disjoint g (singleton_env (fstar_env g) x t) g' })
-  (#e:term)
-  (e_typing:tot_typing g e t)
-  (#e1:st_term) (#c1:comp_st)
-  (e1_typing:st_typing (push_env g (push_env (singleton_env (fstar_env g) x t) g')) e1 c1)
-
-  : st_typing (push_env g (subst_env g' (nt x e)))
-              (subst_st_term e1 (nt x e))
-              (subst_comp c1 (nt x e))
-
-let vprop_equiv_subst
-  (g:env) (x:var) (t:typ) (g':env { pairwise_disjoint g (singleton_env (fstar_env g) x t) g' })
-  (#e:term)
-  (e_typing:tot_typing g e t)
-  (#p1:term) (#p2:term)
-  (veq:vprop_equiv (push_env g (push_env (singleton_env (fstar_env g) x t) g')) p1 p2)
-
-: vprop_equiv (push_env g (subst_env g' (nt x e)))
-              (subst_term p1 (nt x e))
-              (subst_term p2 (nt x e)) =
-  admit ()
+val veq_weakening
+  (g:env) (g':env { disjoint g g' })
+  (#v1 #v2:vprop) (d:vprop_equiv (push_env g g') v1 v2)
+  (g1:env { g1 `env_extends` g /\ disjoint g1 g' })
+  : vprop_equiv (push_env g1 g') v1 v2
